PCP, CFG future proof by Set Default Goal Selector "!".

theories/CFG/Util/Facts.v
@@ -1,5 +1,5 @@
-Require Import List Undecidability.Shared.ListAutomation Lia.
-Import ListNotations ListAutomationNotations.
+Require Import List Lia.
+Import ListNotations.
 
 Fixpoint count (l : list nat) (n : nat)  :=
   match l with
@@ -7,55 +7,51 @@ Fixpoint count (l : list nat) (n : nat)  :=
   | m :: l => if Nat.eqb n m then S (count l n) else count l n
   end.
 
-Lemma countSplit (A B: list nat) (x: nat)  : count A x + count B x = count (A ++ B) x. 
-Proof. 
-  induction A. 
-  - reflexivity. 
-  - cbn. destruct (Nat.eqb x a).
-    + cbn. f_equal; exact IHA. 
-    + exact IHA. 
+Lemma count_count_occ {l n} : count (l : list nat) (n : nat) = count_occ PeanoNat.Nat.eq_dec l n.
+Proof.
+  induction l as [|a l IH]; [reflexivity|].
+  cbn. destruct (PeanoNat.Nat.eq_dec a n) as [->|Han%PeanoNat.Nat.eqb_neq].
+  - now rewrite PeanoNat.Nat.eqb_refl, IH.
+  - now rewrite PeanoNat.Nat.eqb_sym, Han.
+Qed.
+
+Lemma countSplit (A B: list nat) (x: nat) : count A x + count B x = count (A ++ B) x. 
+Proof.
+  now rewrite ?count_count_occ, count_occ_app.
 Qed.
 
 Lemma notInZero (x: nat) A :
-  not (x el A) <-> count A x = 0.
+  not (In x A) <-> count A x = 0.
 Proof.
-  split; induction A.
-  -  reflexivity.
-  - intros H. cbn in *. destruct (PeanoNat.Nat.eqb_spec x a).
-    + exfalso. apply H. left. congruence.
-    + apply IHA. intros F. apply H. now right.
-  - tauto.
-  - cbn. destruct (PeanoNat.Nat.eqb_spec x a).
-    + subst a. lia.
-    + intros H [E | E].
-      * now symmetry in E.
-      * tauto.
+  rewrite ?count_count_occ. now apply count_occ_not_In.
 Qed.
 
-Section fix_X.
-  Variable X:Type.
-  Implicit Types (A B: list X) (a b c: X). 
+Lemma rev_eq {X : Type} (A B: list X):
+  List.rev A = List.rev B <-> A = B.
+Proof.
+  split.
+  - intros H%(f_equal (@rev X)). now rewrite !rev_involutive in H.
+  - now intros <-.
+Qed.
 
-  Lemma last_app_eq A B a b :
-    A++[a] = B++[b] -> A = B /\ a = b.
-  Proof.
-    intros H%(f_equal (@rev X)). rewrite !rev_app_distr in H. split.
-    - inv H. apply (f_equal (@rev X)) in H2. now rewrite !rev_involutive in H2.
-    - now inv H.
-  Qed.
-  
-  Lemma rev_eq A B:
-    List.rev A = List.rev B <-> A = B.
-  Proof.
-    split.
-    - intros H%(f_equal (@rev X)). now rewrite !rev_involutive in H.
-    - now intros <-.
-  Qed.
+Lemma list_prefix_inv X (a : X) x u y v :
+  ~ In a x -> ~ In a u -> x ++ a :: y = u ++ a :: v -> x = u /\ y = v.
+Proof.
+  intro. revert u.
+  induction x; intros; destruct u; inversion H1; subst; try now firstorder.
+  eapply IHx in H4; try now firstorder. intuition congruence.
+Qed.
 
-  Lemma rev_nil A:
-    rev A = [] -> A = [].
-  Proof.
-    destruct A. auto. now intros H%eq_sym%app_cons_not_nil.
-  Qed.
+Fixpoint fresh (l : list nat) :=
+  match l with
+  | [] => 0
+  | x :: l => S x + fresh l
+  end.
 
-End fix_X.
+Lemma fresh_spec (a : nat) (l : list nat) : In a l -> fresh l <> a.
+Proof.
+  intros H. enough (a < fresh l) by lia.
+  revert H. induction l.
+  - easy.
+  - cbn; intros [ | ]; intuition lia.
+Qed.
