theories/CFG/Reductions/PCP_to_CFPP.v
@@ -1,19 +1,17 @@
-Require Import List.
+Require Import List Lia.
 Import ListNotations.
 
 Require Import Undecidability.CFG.CFP.
-Require Import Undecidability.CFG.Util.Facts.
 
 Require Import Undecidability.PCP.PCP.
 Require Import Undecidability.PCP.Util.Facts.
+Import PCPListNotation.
 Require Import Undecidability.PCP.Util.PCP_facts.
 
-Require Import Undecidability.Shared.ListAutomation.
 Require Import Undecidability.Synthetic.Definitions.
 
-Require Import Arith Lia.
-
 Set Default Proof Using "Type".
+Set Default Goal Selector "!".
 
 (* * PCP to CFPP *)
 Section PCP_CFPP.
@@ -76,12 +74,16 @@ Proof.
     exists (gamma A). repeat split.
     + eapply gamma_mono. now rewrite gamma_invol.
     + destruct A; cbn in *; congruence.
-    + eapply tau_eq_iff. intros F % (sym_mono (P := P)) % fresh_spec; now try eapply F. eauto.
+    + eapply tau_eq_iff.
+      * intros F % (sym_mono (P := P)) % fresh_spec; now try eapply F.
+      * eauto.
   - destruct H as (B & Hi & He & H).
     exists (gamma B). repeat split.
     + now eapply gamma_mono.
     + destruct B; cbn in *; congruence.
     + eapply tau_eq_iff with (a := fresh (sym P)).
-      * intros F % (sym_mono (P := P)) % fresh_spec.  now eapply F. now eapply gamma_mono.
+      * intros F % (sym_mono (P := P)) % fresh_spec.
+        ** now eapply F.
+        ** now eapply gamma_mono.
       * rewrite gamma_invol. eassumption.
 Qed.
