theories/PCP/Reductions/SR_to_MPCP.v
@@ -3,6 +3,7 @@ Import ListNotations.
 
 Require Import Undecidability.PCP.PCP.
 Require Import Undecidability.PCP.Util.Facts.
+Import PCPListNotation.
 Require Import Undecidability.PCP.Util.PCP_facts.
 Require Import Undecidability.StringRewriting.SR.
 Require Import Undecidability.StringRewriting.Util.Definitions.
@@ -11,6 +12,7 @@ Require Import Undecidability.Synthetic.Definitions.
 
 Import RuleNotation.
 
+Set Default Goal Selector "!".
 Set Default Proof Using "Type".
 
 (* * SR to MPCP *)
@@ -76,8 +78,8 @@ Section SR_to_MPCP.
     intros. revert H. pattern x; refine (rewt_induct _ _ H0).
     - exists [e]. cbn. firstorder. now simpl_list.
     - clear x H0. intros. inv H. destruct H1 as (A & ? & ?).
-      pose (app_incl_l H2). pose (app_incl_R (app_incl_R H2)).
-      repeat eapply incl_app; try assumption. eauto.
+      { pose (app_incl_l H2). pose (app_incl_R (app_incl_R H2)).
+        repeat eapply incl_app; try assumption. eauto. }
       exists (cards x1 ++ [(u / v)] ++ cards y1 ++ [ [#] / [#] ] ++ A). split.
       + repeat (eapply incl_app); try assumption; unfold P.
         * eapply cards_subset. eapply app_incl_l. eassumption.
@@ -95,12 +97,11 @@ Section SR_to_MPCP.
     intros ?. revert x y. induction A; intros.
     - exfalso. destruct x; inv H2.
     - assert (a el P) as [ -> | [ ->  | [ | [-> | (? & ? & ->)]]]]  % P_inv by (now apply H).
-      + exfalso. cbn -[fresh] in H2. destruct x. inv H2. destruct (sep_doll H4).
+      + exfalso. cbn -[fresh] in H2. destruct x. { inv H2. destruct (sep_doll H4). }
         inversion H2. edestruct doll_sig; eauto.
       + cbn -[fresh] in *.
         autorewrite with list in *. cbn -[fresh] in *.
-        eapply list_prefix_inv in H2 as [<- ?].
-        destruct y.
+        eapply list_prefix_inv in H2 as [<- ?]; [destruct y|..].
         * reflexivity.
         * exfalso. inversion H2. edestruct doll_sig; eauto. 
         * intros E. edestruct hash_sig; eauto.
@@ -108,8 +109,9 @@ Section SR_to_MPCP.
       + destruct a as (u, v).
         cbn -[fresh] in H2.
         edestruct (split_inv H2) as (x' & ->).
-        intros E. edestruct hash_sig. unfold Sigma. rewrite !in_app_iff. do 2 right. now eapply sym_word_l; eauto. reflexivity.
-        econstructor. eapply rewB. now eassumption.        
+        { intros E. edestruct hash_sig. { unfold Sigma. rewrite !in_app_iff. do 2 right. now eapply sym_word_l; eauto. }
+          reflexivity. }
+        econstructor. { eapply rewB. now eassumption. }
         enough ( (y ++ v) ++ x' ≻* y0) by now autorewrite with list in *.
         eapply IHA; autorewrite with list in *.
         * eauto.
@@ -126,7 +128,7 @@ Section SR_to_MPCP.
           eapply IHA. 
           ** eapply cons_incl. eassumption.
           ** eapply cons_incl. eassumption.
-          ** eapply incl_app. eassumption. now eapply ListAutomation.incl_sing.
+          ** eapply incl_app. { eassumption. } now eapply ListAutomation.incl_sing.
           ** simpl_list. eassumption.
   Qed.
 
@@ -135,10 +137,10 @@ Section SR_to_MPCP.
   Proof.
     split.
     - intros ?. cbn in H. eapply SR_MPCP in H as (A & ? & ?).
-      exists A. firstorder. cbn. rewrite H0. cbn. now simpl_list.
+      { exists A. firstorder. cbn. rewrite H0. cbn. now simpl_list. }
       eapply incl_appl. apply incl_refl.
     - intros (A & ? & ?). eapply MPCP_SR with (y := []) (A := A); try trivial.
-      eapply incl_appl. now apply incl_refl.
+      { eapply incl_appl. now apply incl_refl. }
       inv H0. rewrite H2. now simpl_list.
   Qed.
       
